Update most of existing code to new ITree

LeanBoogie/Experimental/State.lean
@@ -37,18 +37,62 @@ def ConA : Con -> Type
 instance : CoeSort Ty Type := ⟨TyA⟩
 instance : CoeSort Con Type := ⟨ConA⟩
 
+set_option linter.unusedVariables false in
+def ConA.get : {Γ : Con} -> Γ -> Var Γ A -> A
+| _ :: _, (x, _), .vz   => x
+| _ :: _, (_, γ), .vs v => γ.get v
+
+set_option linter.unusedVariables false in
+def ConA.update : {Γ : Con} -> Γ -> Var Γ A -> A -> Γ
+| _ :: _, (_, γ), .vz  , a' => (a', γ)
+| _ :: _, (a, γ), .vs v, a' => (a, γ.update v a')
+
+/- ### Normal form of `ConA`
+  Given a starting `γ : ConA Γ` and `γ' = γ.update |>.update .. |>.update ... |> ...`,
+  we can normalize these into essentially `γ' = { #0 := ...γ..., #1 := ...γ..., #2 := ...γ..., ...}`
+  We should have a tactic which performs this normalization in a performant way.
+-/
+@[simp] theorem ConA.update_lww {Γ : Con} {v : Var Γ A} {γ : Γ} : (γ.update v a').update v a'' = γ.update v a'' := sorry
+@[simp] theorem ConA.update_get {Γ : Con} {v : Var Γ A} {γ : Γ} : (γ.update v a').get v = a' := by
+  induction Γ with
+  | nil => cases v
+  | cons B Γ ih =>
+    cases v with
+    | vz => rfl
+    | vs v => simp only [get, ih]
+-- more theorems
+
 -- ## Interaction Tree Events for State
 
-namespace Approach1
-  inductive Mem (Γ : Con) : /- Type -> -/ Type where
-  | rd : Var Γ A          -> Mem Γ /- (TyA A) -/
-  | wr : Var Γ A -> TyA A -> Mem Γ /- Unit -/
-  -- def Mem.read  (v : Var Γ A)           : ITree (Mem Γ) A := .vis (.rd v) (fun a:A => .ret a)
-  -- def Mem.write (v : Var Γ A) (val : A) : ITree (Mem Γ) A := .vis (.wr v val) (fun () => .ret ())
-end Approach1
+inductive Mem (Γ : Con) : Type -> Type where
+| rd : Var Γ A          -> Mem Γ A
+| wr : Var Γ A -> TyA A -> Mem Γ Unit
 
-namespace Approach2
-  inductive Mem (Γ : Type) : /- (A:Type) -> -/ Type where
-  | rd (π : Γ -> Ans) : Mem Γ /- A -/
-  | wr (δ : Γ -> Ans -> Γ) : Mem Γ /- Unit -/
-end Approach2
+def Mem.read  (v : Var Γ A)           : ITree (Mem Γ) A    := .vis (.rd v    ) (fun (a : A) => .ret a)
+def Mem.write (v : Var Γ A) (val : A) : ITree (Mem Γ) Unit := .vis (.wr v val) (fun () => .ret ())
+
+-- ## Example:
+
+structure Global_ where
+  i : Int
+  n : BitVec 32
+
+def Global.Γ : Con := [.int, .bv 32]
+abbrev Global : Type := Global.Γ
+abbrev Global.i (γ : Global) : Int       := γ.get .vz
+abbrev Global.n (γ : Global) : BitVec 32 := γ.get (.vs .vz)
+
+#check Global_.i
+#check Global.i
+
+def Empty' : Type -> Type := fun _ => Empty
+
+inductive Plus (E₁ E₂ : Type -> Type) : Type -> Type
+| left  : E₁ X -> Plus E₁ E₂ X
+| right : E₂ X -> Plus E₁ E₂ X
+
+instance : HAdd (Type -> Type) (Type -> Type) (Type -> Type) := ⟨Plus⟩
+
+def merge : ITree (Mem Γ + Mem Δ) A -> ITree (Mem (Γ ++ Δ)) A := sorry
+
+def interp : ITree (Mem Γ) Unit -> StateT (ConA Γ) (ITree Empty') Unit := sorry
