LeanBoogie/ITree/Iter.lean
@@ -1,0 +1,60 @@
+import LeanBoogie.ITree.ITree
+import LeanBoogie.ITree.Monad
+
+namespace ITree
+
+/-
+  ## ITrees form an *iterative* monad
+-/
+
+
+/-- Repeat a computation until it returns `B`.
+
+  From the ITrees paper, page 12:
+  ```
+  CoFixpoint iter (body : A → itree E (A + B)) : A → itree E B :=
+    fun a ⇒ ab <- body a ;;
+      match ab with
+      | inl a ⇒ Tau (iter body a)
+      | inr b ⇒ Ret b
+      end.
+  ``` -/
+def iter (body : A -> ITree E (A ⊕ B)) (a₀ : A) : ITree E B := sorry -- TODO
+  -- ITree.corec (fun (x : A ⊕ ITree E (B)) =>
+  --   match x with
+  --   | .inl a =>
+  --     -- Run the body, if it returned `a` we iter again, if it returned `b` we are done.
+  --     let res : ITree E (A ⊕ B) := bind (body a) (fun ab =>
+  --       match ab with
+  --       | .inl a => .ret (.inl a)
+  --       | .inr b => .ret (.inr b)
+  --     )
+  --     match res.dest with
+  --     -- | .ret (a : A ⊕ B) => .ret sorry
+  --     | .ret (.inl a) => .tau (.inl a) -- call `iter body a`
+  --     | .ret (.inr b) => .ret b -- we are done
+  --     | .tau (t : ITree E _) => .tau (.inr t)
+  --     | .vis e k => sorry
+  --   | .inr b => Base.replay b .inr
+  -- ) (Sum.inl a₀)
+
+theorem iter_fp {f : A -> ITree E (A ⊕ B)}
+  : iter f a₀ = do let ab <- f a₀
+                   match ab with
+                   | .inl a => (iter f a)
+                   | .inr b => return b
+  := by sorry
+
+/--
+  Definition loop (body : C + A → itree E (C + B)) : A → itree E B :=
+    fun a ⇒ iter (fun ca ⇒
+      cb <- body ca ;;
+      match cb with
+      | inl c ⇒ Ret (inl (inl c))
+      | inr b ⇒ Ret (inr b)
+      end) (inr a).
+-/
+def loop (body : Sum C A -> ITree E (Sum C B)) (a : A) : ITree E B := sorry
+
+def iter_lift (body : A -> ITree E (A ⊕ B)) : (A ⊕ B) -> ITree E (A ⊕ B) :=
+  fun | .inl a => body a | .inr b => return .inr b
