LeanBoogie/ITree/Monad.lean
@@ -1,0 +1,42 @@
+import LeanBoogie.ITree.ITree
+
+namespace ITree
+
+/-
+  # ITrees form a monad
+-/
+
+def pure (a : A) : ITree E A := .ret a
+
+def bind (ta : ITree E A) (tb : A -> ITree E B) : ITree E B := sorry -- TODO: fix
+  -- ITree.corec (β := Sum (ITree E A) (ITree E B)) (fun x =>
+  --   match x with
+  --   | .inl ta =>
+  --     match ta.dest with
+  --     | .ret (.up a : ULift A) =>
+  --       let tb : ITree E B := tb a
+  --       let ret : ITree.Base E B (ITree E B) := tb.dest
+  --       let ret : ITree.Base E B (ITree E A ⊕ ITree E B) := MvFunctor.map (F := TypeFun.ofCurried (n := _) Base) Base.Inr ret
+  --       ret
+  --     | .tau t => .tau (.inl t)
+  --     | .vis e k => .vis e (fun x => .inl (k x))
+  --   | .inr b => Base.replay b Sum.inr
+  -- ) (Sum.inl ta)
+
+instance : Monad (ITree E) where
+  pure := pure
+  bind := bind
+
+instance : LawfulFunctor (ITree E) where
+  map_const := sorry
+  id_map := sorry
+  comp_map := sorry
+
+instance : LawfulMonad (ITree E) where
+  seqLeft_eq := sorry
+  seqRight_eq := sorry
+  pure_seq := sorry
+  bind_pure_comp := sorry
+  bind_map := sorry
+  pure_bind := sorry
+  bind_assoc := sorry
