LeanBoogie/ITree/RunFinite.lean
@@ -1,0 +1,29 @@
+import LeanBoogie.ITree.ITree
+import LeanBoogie.ITree.Monad
+
+namespace ITree
+
+/-- Execute a finite amount of steps of a potentially infinite
+  Returns the events encountered along the way (if any), and the final state (if any).
+  Uses `f` to determine the answer to events. -/
+def runLog (t : ITree E A) (f : ∀Ans, E Ans -> Ans) : Nat -> (List ((Ans : Type) × E Ans)) × Option A
+| 0 => ([], none)
+| n+1 => match t.dest with
+  | .ret (.up a) => ([], some a)
+  | .tau t => runLog t f n
+  | .vis ⟨Ans, .up e, k⟩ => by
+    let t : ITree E A := k (.up (f _ e))
+    let (evs, ret) := runLog t f n
+    exact (⟨Ans, e⟩ :: evs, ret)
+
+/-- Run at most `fuel` steps of `t` in a monad, calling `f` for every event. -/
+def run [Monad m] (t : ITree E A) (fuel : Nat) (f : ∀{Ans}, E Ans -> m Ans) : m (Option A) :=
+  match fuel with
+  | 0 => return none
+  | fuel+1 => match t.dest with
+    | .ret (.up a) => return a
+    | .tau t => run t fuel f
+    | .vis ⟨_, .up e, k⟩ => do
+      let ans <- f e
+      let t : ITree E A := k (.up ans)
+      run t fuel f
