LeanBoogie/Notation.lean
@@ -1,20 +1,20 @@
 
 /-- Two imperative programs executed after one another. Provides the `;; ` notation. -/
-class Seqi (A : Type) where
+class Seqi (A : Type u) where
   seqi : A -> A -> A
 infixl:20 ";; " => Seqi.seqi
 
 /-- Concatenation of continuations. Provides the `>>>` notation. -/
-class Cat (K : Type -> Type -> Type) where
+class Cat (K : Type u -> Type u -> Type u) where
   cat : K A B -> K B C -> K A C
 infixl:75 " >>> " => Cat.cat
 
 /-- Monad morphism from a computation monad `M` to a specification monad `W`. -/
-class Theta (M : Type -> Type) (W : outParam (Type -> Type)) where
+class Theta (M : Type u -> Type u) (W : outParam (Type u -> Type u)) where
   θ : M A -> W A
 export Theta (θ)
 
-class LawfulTheta (M : (Type -> Type)) [m : Monad M] (W : outParam (Type -> Type)) [w : Monad W] [Theta M W] : Prop where
+class LawfulTheta (M : (Type u -> Type u)) [m : Monad M] (W : outParam (Type u -> Type u)) [w : Monad W] [Theta M W] : Prop where
   θ_pure : θ (m.pure a) = w.pure a
   θ_bind : θ (m.bind a b) = w.bind (θ a) (fun a => θ (b a))
 
